ulib/experimental/Steel.ST.Coercions.fst
@@ -1,0 +1,226 @@
+(*
+   Copyright 2020 Microsoft Research
+
+   Licensed under the Apache License, Version 2.0 (the "License");
+   you may not use this file except in compliance with the License.
+   You may obtain a copy of the License at
+
+       http://www.apache.org/licenses/LICENSE-2.0
+
+   Unless required by applicable law or agreed to in writing, software
+   distributed under the License is distributed on an "AS IS" BASIS,
+   WITHOUT WARRANTIES OR CONDITIONS OF ANY KIND, either express or implied.
+   See the License for the specific language governing permissions and
+   limitations under the License.
+*)
+module Steel.ST.Coercions
+(** This module aggregates several of the core effects and utilities
+    associated with the Steel.ST namespace.
+
+    Client modules should typically just [open Steel.ST.Util] and
+    that should bring most of what they need in scope.
+*)
+open FStar.Ghost
+open Steel.Memory
+open Steel.ST.Effect.Ghost
+module U = FStar.Universe
+
+module SF = Steel.Effect
+module SA = Steel.Effect.Atomic
+
+module STF = Steel.ST.Effect
+module STG = Steel.ST.Effect.Ghost
+module STA = Steel.ST.Effect.Atomic
+module STAG = Steel.ST.Effect.AtomicAndGhost
+
+friend Steel.ST.Effect.AtomicAndGhost
+friend Steel.Effect.Atomic
+friend Steel.Effect
+friend Steel.ST.Effect
+friend Steel.ST.Effect.Ghost
+friend Steel.ST.Effect.Atomic
+
+unfold
+let bind_div_st_req (#a:Type) (wp:pure_wp a)
+                    (req_g:a -> Type0)
+  : Type0
+  = FStar.Monotonic.Pure.elim_pure_wp_monotonicity wp;
+    wp (fun _ -> True) /\ (forall x. req_g x)
+
+unfold
+let bind_div_st_ens (#a:Type) (#b:Type)
+                       (wp:pure_wp a)
+                       (ens_g:a -> b -> Type0)
+    : b -> Type0
+    = fun y -> wp (fun _ -> True) /\ (exists x. ens_g x y)
+
+let bind_div_st_ (a:Type) (b:Type)
+                  (#[@@@ framing_implicit] wp:pure_wp a)
+                  (#framed:eqtype_as_type bool)
+                  (#[@@@ framing_implicit] pre:pre_t)
+                  (#[@@@ framing_implicit] post:post_t b)
+                  (#[@@@ framing_implicit] req:a -> Type0)
+                  (#[@@@ framing_implicit] ens:a -> b -> Type0)
+                  (f:eqtype_as_type unit -> DIV a wp)
+                  (g:(x:a -> STF.repr b framed pre post (req x) (ens x)))
+  : STF.repr b
+         framed
+         pre
+         post
+         (bind_div_st_req wp req)
+         (bind_div_st_ens wp ens)
+  = let c
+      : SF.repr b
+                   framed
+                   pre
+                   post
+                   (SF.bind_div_steel_req wp (fun x _ -> req x))
+                   (SF.bind_div_steel_ens wp (fun x _ y _ -> ens x y))
+      =(SF.bind_div_steel a b
+                  wp
+                  framed
+                  pre
+                  post
+                  (fun x _ -> req x)
+                  (fun x _ y _ -> ens x y)
+                  f
+                  g)
+    in
+    FStar.Monotonic.Pure.elim_pure_wp_monotonicity #a wp;
+    STF.weaken_repr _ _ _ _ _ _ _ _ c () ()
+
+polymonadic_bind (DIV, STF.STBase) |> STF.STBase = bind_div_st_
+
+let reify_steel_comp (#a:Type)
+                     (#pre:pre_t)
+                     (#post:post_t a)
+                     (#req:Type0)
+                     (#ens:a -> Type0)
+                     ($f:unit -> SF.SteelBase a false pre post (fun _ -> req) (fun _ x _ -> ens x))
+  : Dv (STF.repr a false pre post req ens)
+  = SF.reify_steel_comp f
+
+let reflect (#a:Type)
+            (#pre:pre_t)
+            (#post:post_t a)
+            (#req:Type0)
+            (#ens:a -> Type0)
+            ($f:STF.repr a false pre post req ens)
+  : STF.ST a pre post req ens
+  = STF.STBase?.reflect f
+
+let coerce_steel (#a:Type)
+                 (#pre:pre_t)
+                 (#post:post_t a)
+                 (#req:st_req_t)
+                 (#ens:st_ens_t a)
+                 ($f:unit -> SF.SteelBase a false pre post
+                          (fun _ -> req)
+                          (fun _ x _ -> ens x))
+   : STF.ST a pre post req ens
+   = reflect (reify_steel_comp f)
+
+let coerce_atomic #a #o #obs
+                 (#p:vprop)
+                 (#q:a -> vprop)
+                 (#pre:Type0)
+                 (#post: a -> Type0)
+                 ($f:unit -> SA.SteelAtomicBase a false o obs p q
+                   (fun _ -> pre)
+                   (fun _ x _ -> post x))
+  : STA.STAtomicBase a false o obs p q pre post
+  = STA.STAtomicBase?.reflect (SA.reify_steel_atomic_comp f)
+
+let coerce_atomicF #a #o #p #q #pre #post f
+  = STA.STAtomicBase?.reflect (SA.reify_steel_atomic_comp f)
+
+let coerce_ghost (#a:Type)
+                 (#o:inames)
+                 (#p:vprop)
+                 (#q:a -> vprop)
+                 (#pre:Type0)
+                 (#post: a -> Type0)
+                 ($f:unit -> SA.SteelGhostBase a false o Unobservable p q
+                   (fun _ -> pre)
+                   (fun _ x _ -> post x))
+  : STG.STGhostBase a false o Unobservable p q pre post
+  = STG.STGhostBase?.reflect (SA.reify_steel_ghost_comp f)
+
+let coerce_ghostF #a #o #p #q #pre #post f
+  = STGhostBase?.reflect (SA.reify_steel_ghost_comp f)
+
+let lift_st_steel
+      (a:Type)
+      (#framed:eqtype_as_type bool)
+      (#pre:pre_t)
+      (#post:post_t a)
+      (#req:Type0)
+      (#ens:a -> Type0)
+      (f:STF.repr a framed pre post req ens)
+  : SF.repr a framed pre post (fun _ -> req) (fun _ x _ -> ens x)
+  = f
+
+
+let lift_sta_sa
+      (a:Type)
+      (#framed:eqtype_as_type bool)
+      (#o:inames)
+      (#obs:eqtype_as_type observability)
+      (#pre:pre_t)
+      (#post:post_t a)
+      (#req:Type0)
+      (#ens:a -> Type0)
+      (f:STAG.repr a framed o obs pre post req ens)
+  : SA.repr a framed o obs pre post (fun _ -> req) (fun _ x _ -> ens x)
+  = f
+
+
+let lift_stag_sa
+      (a:Type)
+      (#framed:eqtype_as_type bool)
+      (#o:inames)
+      (#obs:eqtype_as_type observability)
+      (#pre:pre_t)
+      (#post:post_t a)
+      (#req:Type0)
+      (#ens:a -> Type0)
+      (f:STAG.repr a framed o obs pre post req ens)
+  : SA.repr a framed o obs pre post (fun _ -> req) (fun _ x _ -> ens x)
+  = f
+
+let lift_stg_steelg (#a:Type)
+                     #o #p
+                     (#q:a -> vprop)
+                     (#pre:Type0)
+                     (#post: a -> Type0)
+                     (f:unit -> STGhost a o p q pre post)
+                     (_:unit)
+  : SA.SteelGhost a o p q (fun _ -> pre) (fun _ x _ -> post x)
+  = f()
+
+(* I would like to define this, but I cannot
+   because of an effect ordering constraint *)
+// sub_effect STA.STAtomicBase ~> SA.SteelAtomicBase = lift_sta_sa
+
+(* So, instead, I assume a reification of STAtomicBase *)
+assume
+val reify_st_atomic_base(#a:Type)
+                        (#framed:eqtype_as_type bool)
+                        (#obs:eqtype_as_type observability)
+                        (#o:inames)
+                        (#p:vprop)
+                        (#q:a -> vprop)
+                        (#pre:Type0)
+                        (#post: a -> Type0)
+                        ($f:unit -> STA.STAtomicBase a framed o obs p q pre post)
+  : STAG.repr a framed o obs p q pre post
+
+let lift_sta_steela (#a:Type)
+                     #o #p
+                     (#q:a -> vprop)
+                     (#pre:Type0)
+                     (#post: a -> Type0)
+                     (f:unit -> STA.STAtomic a o p q pre post)
+                     (_:unit)
+  : SA.SteelAtomic a o p q (fun _ -> pre) (fun _ x _ -> post x)
+  = SA.SteelAtomicBase?.reflect (reify_st_atomic_base f)
