ulib/experimental/Steel.ST.SpinLock.fsti
@@ -18,9 +18,10 @@ module Steel.ST.SpinLock
 open Steel.ST.Util
 
 /// A Steel library to share resources between threads through locks.
+/// It is implemented on top of Steel.SpinLock
 
-/// The type of a lock.
-/// This is implemented as a pair of a boolean reference, and an invariant name
+/// The type of a lock.  This is implemented as a pair of a boolean
+/// reference, and an invariant name
 val lock_t : Type u#0
 
 /// A predicate relating a lock to a vprop.
@@ -30,16 +31,17 @@ val protects (l:lock_t) (p:vprop) : prop
 let lock (p:vprop) = l:lock_t{l `protects` p}
 
 /// If we have vprop [p] in the context, we can create a new lock
-/// associated to [p]. [p] is then removed from the context, and only accessible
-/// through the newly created lock
+/// associated to [p]. [p] is then removed from the context, and only
+/// accessible through the newly created lock
 val new_lock (p:vprop)
   : STT (lock p) p (fun _ -> emp)
 
-/// Acquires the lock, and adds the associated vprop [p] to the context.
-/// This function loops until the lock becomes available
+/// Acquires the lock, and adds the associated vprop [p] to the
+/// context. This function loops until the lock becomes available
 val acquire (#p:vprop) (l:lock p)
   : STT unit emp (fun _ -> p)
 
-/// Releases a lock [l], as long as the caller previously restored the associated vprop [p]
+/// Releases a lock [l], as long as the caller previously restored the
+/// associated vprop [p]
 val release (#p:vprop) (l:lock p)
   : STT unit p (fun _ -> emp)
